extractor: add rev-normalized satisfies_constraint lemmas

src/Extractor.v
@@ -16,8 +16,19 @@ Require Import Lia.
 Require Import LibTactics.
 Require Import sflib.
 Require Import Misc.
+Require Import Validator.
+Require Import Permutation.
+Require Import Sorting.Sorted.
 
 Module Extractor (PolIRs: POLIRS).
+
+Module Instr := PolIRs.Instr.
+Module State := PolIRs.State.
+Module Ty := PolIRs.Ty.
+Module PolyLang := PolIRs.PolyLang.
+Module Loop := PolIRs.Loop.
+Module Val := Validator PolIRs.
+Definition ident := Instr.ident.
 
 (* Note: empty domain contains exactly one instance: [] (empty list) *)
 
@@ -46,6 +57,108 @@ Fixpoint expr_to_aff (e: PolIRs.Loop.expr): result (list Z * Z) :=
         end
     | _ => Err "Expr to aff failed."%string
     end.
+
+Fixpoint wf_affine_expr (e: PolIRs.Loop.expr): bool :=
+    match e with
+    | PolIRs.Loop.Constant _ => true
+    | PolIRs.Loop.Var _ => true
+    | PolIRs.Loop.Mult _ e' => wf_affine_expr e'
+    | PolIRs.Loop.Sum e1 e2 => wf_affine_expr e1 && wf_affine_expr e2
+    | _ => false
+    end.
+
+Fixpoint wf_affine_expr_list (es: list PolIRs.Loop.expr): bool :=
+    match es with
+    | [] => true
+    | e :: es' => wf_affine_expr e && wf_affine_expr_list es'
+    end.
+
+Fixpoint wf_affine_test (tst: PolIRs.Loop.test): bool :=
+    match tst with
+    | PolIRs.Loop.LE e1 e2 => wf_affine_expr e1 && wf_affine_expr e2
+    | PolIRs.Loop.EQ e1 e2 => wf_affine_expr e1 && wf_affine_expr e2
+    | PolIRs.Loop.And t1 t2 => wf_affine_test t1 && wf_affine_test t2
+    | _ => false
+    end.
+
+Fixpoint wf_scop_stmt (stmt: PolIRs.Loop.stmt): bool :=
+    match stmt with
+    | PolIRs.Loop.Instr _ es => wf_affine_expr_list es
+    | PolIRs.Loop.Seq stmts => wf_scop_stmts stmts
+    | PolIRs.Loop.Loop lb ub body =>
+        wf_affine_expr lb && wf_affine_expr ub && wf_scop_stmt body
+    | PolIRs.Loop.Guard test body =>
+        wf_affine_test test && wf_scop_stmt body
+    end
+with wf_scop_stmts (stmts: PolIRs.Loop.stmt_list): bool :=
+    match stmts with
+    | PolIRs.Loop.SNil => true
+    | PolIRs.Loop.SCons stmt stmts' => wf_scop_stmt stmt && wf_scop_stmts stmts'
+    end.
+
+Lemma andb_true_iff_local0:
+    forall b1 b2, (b1 && b2)%bool = true <-> b1 = true /\ b2 = true.
+Proof.
+    intros b1 b2. destruct b1, b2; simpl; tauto.
+Qed.
+
+Lemma wf_scop_instr_inv:
+    forall instr es,
+    wf_scop_stmt (PolIRs.Loop.Instr instr es) = true ->
+    wf_affine_expr_list es = true.
+Proof.
+    intros instr es Hwf.
+    simpl in Hwf. exact Hwf.
+Qed.
+
+Lemma wf_scop_seq_inv:
+    forall stmts,
+    wf_scop_stmt (PolIRs.Loop.Seq stmts) = true ->
+    wf_scop_stmts stmts = true.
+Proof.
+    intros stmts Hwf.
+    simpl in Hwf. exact Hwf.
+Qed.
+
+Lemma wf_scop_loop_inv:
+    forall lb ub body,
+    wf_scop_stmt (PolIRs.Loop.Loop lb ub body) = true ->
+    wf_affine_expr lb = true /\
+    wf_affine_expr ub = true /\
+    wf_scop_stmt body = true.
+Proof.
+    intros lb ub body Hwf.
+    simpl in Hwf.
+    eapply andb_true_iff_local0 in Hwf.
+    destruct Hwf as [Hlbub Hbody].
+    eapply andb_true_iff_local0 in Hlbub.
+    destruct Hlbub as [Hlb Hub].
+    repeat split; auto.
+Qed.
+
+Lemma wf_scop_guard_inv:
+    forall test body,
+    wf_scop_stmt (PolIRs.Loop.Guard test body) = true ->
+    wf_affine_test test = true /\
+    wf_scop_stmt body = true.
+Proof.
+    intros test body Hwf.
+    simpl in Hwf.
+    eapply andb_true_iff_local0 in Hwf.
+    exact Hwf.
+Qed.
+
+Lemma wf_scop_stmts_cons_inv:
+    forall stmt stmts',
+    wf_scop_stmts (PolIRs.Loop.SCons stmt stmts') = true ->
+    wf_scop_stmt stmt = true /\
+    wf_scop_stmts stmts' = true.
+Proof.
+    intros stmt stmts' Hwf.
+    simpl in Hwf.
+    eapply andb_true_iff_local0 in Hwf.
+    exact Hwf.
+Qed.
 
 Lemma expr_to_aff_correct: 
     forall e env aff v z, expr_to_aff e = Okk aff -> 
@@ -121,20 +234,317 @@ Example test_expr_to_aff_6:
     = Okk ([0%Z; 0%Z; 0%Z; 1%Z; 2%Z], 5%Z).
 Proof. reflexivity. Qed.
 
-Fixpoint exprlist_to_aff (es: list PolIRs.Loop.expr) (depth: nat): result (list (list Z * Z)) 
+Fixpoint exprlist_to_aff (es: list PolIRs.Loop.expr) (cols: nat): result (list (list Z * Z))
 := 
     match es with 
     | [] => Okk []
     | e :: es' => 
         match (expr_to_aff e) with 
-        | Okk aff => 
-            match (exprlist_to_aff es' depth) with 
+        | Okk (v, c) =>
+            let aff := (resize cols v, c) in
+            match (exprlist_to_aff es' cols) with
             | Okk affs => Okk (aff :: affs)
             | Err msg => Err msg
             end
         | Err msg => Err msg
         end
     end.
+
+Lemma exprlist_to_aff_length:
+    forall es cols affs,
+    exprlist_to_aff es cols = Okk affs ->
+    Datatypes.length affs = Datatypes.length es.
+Proof.
+    induction es; intros cols affs H; simpl in H.
+    - inv H. auto.
+    - destruct (expr_to_aff a) as [[v c]|msg] eqn:Ha; try discriminate.
+      destruct (exprlist_to_aff es cols) as [affs'|msg'] eqn:Hes; try discriminate.
+      inv H. simpl.
+      eapply IHes in Hes.
+      lia.
+Qed.
+
+Lemma exprlist_to_aff_rows_cols:
+    forall es cols affs,
+    exprlist_to_aff es cols = Okk affs ->
+    Forall (fun aff => Datatypes.length (fst aff) = cols) affs.
+Proof.
+    induction es; intros cols affs H; simpl in H.
+    - inv H. constructor.
+    - destruct (expr_to_aff a) as [[v c]|msg] eqn:Ha; try discriminate.
+      destruct (exprlist_to_aff es cols) as [affs'|msg'] eqn:Hes; try discriminate.
+      inv H.
+      constructor.
+      + simpl. eapply resize_length.
+      + eapply IHes; eauto.
+Qed.
+
+Lemma exprlist_to_aff_correct:
+    forall es env cols affs,
+    exprlist_to_aff es cols = Okk affs ->
+    Datatypes.length env = cols ->
+    map (Loop.eval_expr env) es = affine_product affs env.
+Proof.
+    induction es as [|e es IH]; intros env cols affs Haff Hlen; simpl in Haff.
+    - inversion Haff; clear Haff; subst affs. reflexivity.
+    - destruct (expr_to_aff e) as [[v c]|msg] eqn:He; try discriminate.
+      destruct (exprlist_to_aff es cols) as [affs'|msg'] eqn:Hes; try discriminate.
+      pose proof Hlen as Hlen0.
+      inversion Haff; clear Haff; subst affs. simpl.
+      f_equal.
+      + pose proof (expr_to_aff_correct e env (v, c) v c He eq_refl) as Heval.
+        simpl.
+        rewrite Heval.
+        rewrite dot_product_commutative.
+        assert (dot_product (resize cols v) env = dot_product v env) as Hdot.
+        { rewrite <- Hlen0. rewrite dot_product_resize_left. reflexivity. }
+        rewrite Hdot.
+        reflexivity.
+      + eapply IH; eauto.
+Qed.
+
+Definition normalize_affine (cols: nat) (aff: list Z * Z): (list Z * Z) :=
+    let (v, c) := aff in (resize cols v, c).
+
+Definition normalize_affine_list (cols: nat) (affs: list (list Z * Z)) :=
+    map (normalize_affine cols) affs.
+
+Definition normalize_access (cols: nat) (acc: AccessFunction): AccessFunction :=
+    let (arrid, affs) := acc in (arrid, normalize_affine_list cols affs).
+
+Definition normalize_access_list (cols: nat) (accs: list AccessFunction) :=
+    map (normalize_access cols) accs.
+
+Definition normalize_affine_rev (cols: nat) (aff: list Z * Z): (list Z * Z) :=
+    let (v, c) := aff in (rev (resize cols v), c).
+
+Definition normalize_affine_list_rev (cols: nat) (affs: list (list Z * Z)) :=
+    map (normalize_affine_rev cols) affs.
+
+Definition normalize_access_rev (cols: nat) (acc: AccessFunction): AccessFunction :=
+    let (arrid, affs) := acc in (arrid, normalize_affine_list_rev cols affs).
+
+Definition normalize_access_list_rev (cols: nat) (accs: list AccessFunction) :=
+    map (normalize_access_rev cols) accs.
+
+Lemma normalize_affine_satisfies_constraint:
+    forall cols env aff,
+    Datatypes.length env = cols ->
+    satisfies_constraint env (normalize_affine cols aff) =
+    satisfies_constraint env aff.
+Proof.
+    intros cols env [v c] Hlen.
+    unfold normalize_affine. simpl.
+    unfold satisfies_constraint. simpl.
+    rewrite <- Hlen.
+    rewrite dot_product_resize_right.
+    reflexivity.
+Qed.
+
+Lemma normalize_affine_list_satisfies_constraint:
+    forall cols env affs,
+    Datatypes.length env = cols ->
+    forallb (satisfies_constraint env) (normalize_affine_list cols affs) =
+    forallb (satisfies_constraint env) affs.
+Proof.
+    intros cols env affs Hlen.
+    induction affs as [|aff affs IH]; simpl.
+    - reflexivity.
+    - rewrite normalize_affine_satisfies_constraint with (cols:=cols) (env:=env) (aff:=aff) by auto.
+      f_equal. exact IH.
+Qed.
+
+Lemma normalize_affine_eval:
+    forall cols env aff,
+    Datatypes.length env = cols ->
+    dot_product (fst (normalize_affine cols aff)) env + snd (normalize_affine cols aff) =
+    dot_product (fst aff) env + snd aff.
+Proof.
+    intros cols env [v c] Hlen.
+    unfold normalize_affine. simpl.
+    rewrite <- Hlen.
+    rewrite dot_product_resize_left.
+    lia.
+Qed.
+
+Lemma normalize_affine_list_affine_product:
+    forall cols env affs,
+    Datatypes.length env = cols ->
+    affine_product (normalize_affine_list cols affs) env = affine_product affs env.
+Proof.
+    intros cols env affs Hlen.
+    induction affs as [|aff affs IH]; simpl.
+    - reflexivity.
+    - f_equal.
+      + eapply normalize_affine_eval; eauto.
+      + exact IH.
+Qed.
+
+Lemma dot_product_rev:
+    forall xs ys,
+    Datatypes.length xs = Datatypes.length ys ->
+    dot_product (rev xs) (rev ys) = dot_product xs ys.
+Proof.
+    induction xs as [|x xs IH]; intros ys Hlen.
+    - destruct ys; simpl in *; [reflexivity|lia].
+    - destruct ys as [|y ys]; simpl in *; [lia|].
+      inversion Hlen as [Hlen'].
+      rewrite !dot_product_app.
+      2: rewrite !rev_length; simpl; lia.
+      simpl.
+      rewrite IH; [lia|exact Hlen'].
+Qed.
+
+Lemma dot_product_env_rev_vec:
+    forall env v,
+    Datatypes.length env = Datatypes.length v ->
+    dot_product env (rev v) = dot_product (rev env) v.
+Proof.
+    intros env v Hlen.
+    pose proof (dot_product_rev env (rev v)) as Hrev.
+    assert (Datatypes.length env = Datatypes.length (rev v)) as Hlen'.
+    { rewrite rev_length; exact Hlen. }
+    specialize (Hrev Hlen').
+    rewrite rev_involutive in Hrev.
+    symmetry.
+    exact Hrev.
+Qed.
+
+Lemma normalize_affine_rev_eval:
+    forall cols env aff,
+    Datatypes.length env = cols ->
+    dot_product (fst (normalize_affine_rev cols aff)) env + snd (normalize_affine_rev cols aff) =
+    dot_product (fst aff) (rev env) + snd aff.
+Proof.
+    intros cols env [v c] Hlen.
+    unfold normalize_affine_rev. simpl.
+    rewrite dot_product_commutative.
+    rewrite dot_product_env_rev_vec.
+    2: rewrite resize_length; exact Hlen.
+    rewrite dot_product_commutative.
+    assert (Datatypes.length (rev env) = cols) as Hlenrev.
+    { rewrite rev_length; exact Hlen. }
+    rewrite <- Hlenrev at 1.
+    rewrite dot_product_resize_left.
+    lia.
+Qed.
+
+Lemma normalize_affine_list_rev_affine_product:
+    forall cols env affs,
+    Datatypes.length env = cols ->
+    affine_product (normalize_affine_list_rev cols affs) env = affine_product affs (rev env).
+Proof.
+    intros cols env affs Hlen.
+    induction affs as [|aff affs IH]; simpl.
+    - reflexivity.
+    - f_equal.
+      + eapply normalize_affine_rev_eval; eauto.
+      + exact IH.
+Qed.
+
+Lemma normalize_affine_rev_satisfies_constraint:
+    forall cols env aff,
+    Datatypes.length env = cols ->
+    satisfies_constraint env (normalize_affine_rev cols aff) =
+    satisfies_constraint (rev env) aff.
+Proof.
+    intros cols env [v c] Hlen.
+    unfold normalize_affine_rev. simpl.
+    unfold satisfies_constraint. simpl.
+    rewrite dot_product_env_rev_vec.
+    2: rewrite resize_length; exact Hlen.
+    rewrite dot_product_commutative.
+    assert (Datatypes.length (rev env) = cols) as Hlenrev.
+    { rewrite rev_length; exact Hlen. }
+    rewrite <- Hlenrev at 1.
+    rewrite dot_product_resize_left.
+    rewrite dot_product_commutative.
+    reflexivity.
+Qed.
+
+Lemma normalize_affine_list_rev_satisfies_constraint:
+    forall cols env affs,
+    Datatypes.length env = cols ->
+    forallb (satisfies_constraint env) (normalize_affine_list_rev cols affs) =
+    forallb (satisfies_constraint (rev env)) affs.
+Proof.
+    intros cols env affs Hlen.
+    induction affs as [|aff affs IH]; simpl.
+    - reflexivity.
+    - rewrite normalize_affine_rev_satisfies_constraint with (cols:=cols) (env:=env) (aff:=aff) by auto.
+      f_equal. exact IH.
+Qed.
+
+Lemma exprlist_to_aff_normalized_correct:
+    forall es env cols tf,
+    exprlist_to_aff es cols = Okk tf ->
+    Datatypes.length env = cols ->
+    affine_product (normalize_affine_list cols tf) env = map (Loop.eval_expr env) es.
+Proof.
+    intros es env cols tf Htf Hlen.
+    rewrite normalize_affine_list_affine_product with (cols:=cols) (env:=env) (affs:=tf); auto.
+    symmetry.
+    eapply exprlist_to_aff_correct; eauto.
+Qed.
+
+Lemma exprlist_to_aff_rev_normalized_correct:
+    forall es env cols tf,
+    exprlist_to_aff es cols = Okk tf ->
+    Datatypes.length env = cols ->
+    affine_product (normalize_affine_list_rev cols tf) env = map (Loop.eval_expr (rev env)) es.
+Proof.
+    intros es env cols tf Htf Hlen.
+    rewrite normalize_affine_list_rev_affine_product with (cols:=cols) (env:=env) (affs:=tf); auto.
+    symmetry.
+    eapply exprlist_to_aff_correct; eauto.
+    rewrite rev_length; exact Hlen.
+Qed.
+
+Definition resolve_access_functions
+    (instr: Instr.t) : option (list AccessFunction * list AccessFunction) :=
+    let empty := (@nil AccessFunction) in
+    match PolIRs.Instr.waccess instr, PolIRs.Instr.raccess instr with
+    | Some w, Some r =>
+        if PolIRs.Instr.access_function_checker w r instr
+        then Some (w, r)
+        else None
+    | Some w, None =>
+        if PolIRs.Instr.access_function_checker w empty instr
+        then Some (w, empty)
+        else None
+    | None, Some r =>
+        if PolIRs.Instr.access_function_checker empty r instr
+        then Some (empty, r)
+        else None
+    | None, None =>
+        if PolIRs.Instr.access_function_checker empty empty instr
+        then Some (empty, empty)
+        else None
+    end.
+
+Lemma resolve_access_functions_sound:
+    forall instr w r,
+    resolve_access_functions instr = Some (w, r) ->
+    Instr.valid_access_function w r instr.
+Proof.
+    intros instr w r Hres.
+    unfold resolve_access_functions in Hres.
+    remember (PolIRs.Instr.waccess instr) as wopt.
+    remember (PolIRs.Instr.raccess instr) as ropt.
+    destruct wopt as [w0|]; destruct ropt as [r0|]; simpl in Hres.
+    - destruct (PolIRs.Instr.access_function_checker w0 r0 instr) eqn:Hcheck; try discriminate.
+      inv Hres.
+      eapply PolIRs.Instr.access_function_checker_correct; eauto.
+    - destruct (PolIRs.Instr.access_function_checker w0 [] instr) eqn:Hcheck; try discriminate.
+      inv Hres.
+      eapply PolIRs.Instr.access_function_checker_correct; eauto.
+    - destruct (PolIRs.Instr.access_function_checker [] r0 instr) eqn:Hcheck; try discriminate.
+      inv Hres.
+      eapply PolIRs.Instr.access_function_checker_correct; eauto.
+    - destruct (PolIRs.Instr.access_function_checker [] [] instr) eqn:Hcheck; try discriminate.
+      inv Hres.
+      eapply PolIRs.Instr.access_function_checker_correct; eauto.
+Qed.
 
 Definition make_le_constr (aff1 aff2: list Z * Z): list Z * Z := 
     let (aff1, c1) := aff1 in 
@@ -161,6 +571,56 @@ Example test_make_ge_constr:
     = ([1%Z; 0%Z; 1%Z], 0%Z).
 Proof. reflexivity. Qed.
 
+Lemma dot_product_opp_right:
+    forall p v,
+    dot_product p (map Z.opp v) = Z.opp (dot_product p v).
+Proof.
+    induction p as [|x p IH]; intros v; destruct v as [|y v']; simpl; try lia.
+    rewrite IH. lia.
+Qed.
+
+Lemma make_le_constr_correct:
+    forall env aff1 aff2,
+    satisfies_constraint env (make_le_constr aff1 aff2) = true <->
+    let (v1, c1) := aff1 in
+    let (v2, c2) := aff2 in
+    (dot_product env v1 + c1 <= dot_product env v2 + c2)%Z.
+Proof.
+    intros env [v1 c1] [v2 c2]. simpl.
+    unfold satisfies_constraint. simpl.
+    rewrite add_vector_dot_product_distr_right.
+    rewrite dot_product_opp_right.
+    rewrite Z.leb_le.
+    lia.
+Qed.
+
+Lemma make_ge_constr_correct:
+    forall env aff1 aff2,
+    satisfies_constraint env (make_ge_constr aff1 aff2) = true <->
+    let (v1, c1) := aff1 in
+    let (v2, c2) := aff2 in
+    (dot_product env v2 + c2 <= dot_product env v1 + c1)%Z.
+Proof.
+    intros env [v1 c1] [v2 c2]. simpl.
+    unfold satisfies_constraint. simpl.
+    rewrite add_vector_dot_product_distr_right.
+    rewrite dot_product_opp_right.
+    rewrite Z.leb_le.
+    lia.
+Qed.
+
+Lemma andb_true_r_local:
+    forall b, (b && true)%bool = b.
+Proof.
+    destruct b; reflexivity.
+Qed.
+
+Lemma andb_true_iff_local:
+    forall b1 b2, (b1 && b2)%bool = true <-> b1 = true /\ b2 = true.
+Proof.
+    intros b1 b2. destruct b1, b2; simpl; tauto.
+Qed.
+
 
 (** test to constraint *)
 Fixpoint test_to_aff (tst: PolIRs.Loop.test): result (list (list Z * Z)) := 
@@ -186,6 +646,246 @@ Fixpoint test_to_aff (tst: PolIRs.Loop.test): result (list (list Z * Z)) :=
     | _ => Err "Test to aff failed"%string
     end.
 
+Lemma test_to_aff_sound:
+    forall tst env constrs,
+    test_to_aff tst = Okk constrs ->
+    Loop.eval_test env tst = true ->
+    forallb (satisfies_constraint env) constrs = true.
+Proof.
+    induction tst as [e1 e2|e1 e2|tst1 IH1 tst2 IH2|tst1 IH1 tst2 IH2|tst IH|b];
+      intros env constrs Htst Heval; simpl in *; try discriminate.
+    - destruct (expr_to_aff e1) as [[v1 c1]|msg1] eqn:He1; try discriminate.
+      destruct (expr_to_aff e2) as [[v2 c2]|msg2] eqn:He2; try discriminate.
+      inv Htst.
+      apply Z.leb_le in Heval.
+      pose proof (expr_to_aff_correct e1 env (v1, c1) v1 c1 He1 eq_refl) as Hv1.
+      pose proof (expr_to_aff_correct e2 env (v2, c2) v2 c2 He2 eq_refl) as Hv2.
+      rewrite Hv1 in Heval. rewrite Hv2 in Heval.
+      simpl. rewrite andb_true_r_local.
+      eapply (proj2 (make_le_constr_correct env (v1, c1) (v2, c2))).
+      lia.
+    - destruct (expr_to_aff e1) as [[v1 c1]|msg1] eqn:He1; try discriminate.
+      destruct (expr_to_aff e2) as [[v2 c2]|msg2] eqn:He2; try discriminate.
+      inv Htst.
+      apply Z.eqb_eq in Heval.
+      pose proof (expr_to_aff_correct e1 env (v1, c1) v1 c1 He1 eq_refl) as Hv1.
+      pose proof (expr_to_aff_correct e2 env (v2, c2) v2 c2 He2 eq_refl) as Hv2.
+      rewrite Hv1 in Heval. rewrite Hv2 in Heval.
+      simpl. rewrite andb_true_r_local.
+      rewrite andb_true_iff_local. split.
+      + eapply (proj2 (make_le_constr_correct env (v1, c1) (v2, c2))). lia.
+      + eapply (proj2 (make_ge_constr_correct env (v1, c1) (v2, c2))). lia.
+    - destruct (test_to_aff tst1) as [cs1|msg1] eqn:H1; try discriminate.
+      destruct (test_to_aff tst2) as [cs2|msg2] eqn:H2; try discriminate.
+      inv Htst.
+      apply andb_true_iff_local in Heval. destruct Heval as [Hv1 Hv2].
+      rewrite forallb_app. rewrite andb_true_iff_local. split.
+      + eapply IH1; eauto.
+      + eapply IH2; eauto.
+Qed.
+
+Lemma test_to_aff_complete:
+    forall tst env constrs,
+    test_to_aff tst = Okk constrs ->
+    forallb (satisfies_constraint env) constrs = true ->
+    Loop.eval_test env tst = true.
+Proof.
+    induction tst as [e1 e2|e1 e2|tst1 IH1 tst2 IH2|tst1 IH1 tst2 IH2|tst IH|b];
+      intros env constrs Htst Hsat; simpl in *; try discriminate.
+    - destruct (expr_to_aff e1) as [[v1 c1]|msg1] eqn:He1; try discriminate.
+      destruct (expr_to_aff e2) as [[v2 c2]|msg2] eqn:He2; try discriminate.
+      inv Htst.
+      simpl in Hsat.
+      rewrite andb_true_r_local in Hsat.
+      eapply (proj1 (make_le_constr_correct env (v1, c1) (v2, c2))) in Hsat.
+      eapply Z.leb_le.
+      pose proof (expr_to_aff_correct e1 env (v1, c1) v1 c1 He1 eq_refl) as Hv1.
+      pose proof (expr_to_aff_correct e2 env (v2, c2) v2 c2 He2 eq_refl) as Hv2.
+      rewrite Hv1, Hv2.
+      exact Hsat.
+    - destruct (expr_to_aff e1) as [[v1 c1]|msg1] eqn:He1; try discriminate.
+      destruct (expr_to_aff e2) as [[v2 c2]|msg2] eqn:He2; try discriminate.
+      inv Htst.
+      simpl in Hsat.
+      rewrite andb_true_r_local in Hsat.
+      eapply andb_true_iff_local in Hsat.
+      destruct Hsat as [Hle Hge].
+      eapply (proj1 (make_le_constr_correct env (v1, c1) (v2, c2))) in Hle.
+      eapply (proj1 (make_ge_constr_correct env (v1, c1) (v2, c2))) in Hge.
+      eapply Z.eqb_eq.
+      pose proof (expr_to_aff_correct e1 env (v1, c1) v1 c1 He1 eq_refl) as Hv1.
+      pose proof (expr_to_aff_correct e2 env (v2, c2) v2 c2 He2 eq_refl) as Hv2.
+      rewrite Hv1, Hv2.
+      lia.
+    - destruct (test_to_aff tst1) as [cs1|msg1] eqn:H1; try discriminate.
+      destruct (test_to_aff tst2) as [cs2|msg2] eqn:H2; try discriminate.
+      inv Htst.
+      rewrite forallb_app in Hsat.
+      eapply andb_true_iff_local in Hsat.
+      destruct Hsat as [Hs1 Hs2].
+      simpl.
+      specialize (IH1 env cs1 eq_refl Hs1).
+      specialize (IH2 env cs2 eq_refl Hs2).
+      rewrite IH1.
+      rewrite IH2.
+      reflexivity.
+Qed.
+
+Lemma test_to_aff_sound_normalized:
+    forall tst env cols constrs,
+    test_to_aff tst = Okk constrs ->
+    Loop.eval_test env tst = true ->
+    Datatypes.length env = cols ->
+    forallb (satisfies_constraint env) (normalize_affine_list cols constrs) = true.
+Proof.
+    intros tst env cols constrs Htst Heval Hlen.
+    rewrite normalize_affine_list_satisfies_constraint with (cols:=cols) (env:=env) (affs:=constrs); auto.
+    eapply test_to_aff_sound; eauto.
+Qed.
+
+Lemma test_to_aff_complete_normalized:
+    forall tst env cols constrs,
+    test_to_aff tst = Okk constrs ->
+    Datatypes.length env = cols ->
+    forallb (satisfies_constraint env) (normalize_affine_list cols constrs) = true ->
+    Loop.eval_test env tst = true.
+Proof.
+    intros tst env cols constrs Htst Hlen Hsat.
+    rewrite normalize_affine_list_satisfies_constraint with (cols:=cols) (env:=env) (affs:=constrs) in Hsat; auto.
+    eapply test_to_aff_complete; eauto.
+Qed.
+
+Lemma test_false_implies_not_in_poly_normalized:
+    forall tst env cols constrs,
+    test_to_aff tst = Okk constrs ->
+    Datatypes.length env = cols ->
+    Loop.eval_test env tst = false ->
+    in_poly env (normalize_affine_list cols constrs) = false.
+Proof.
+    intros tst env cols constrs Htst Hlen Heval.
+    unfold in_poly.
+    destruct (forallb (satisfies_constraint env) (normalize_affine_list cols constrs)) eqn:HSat.
+    - exfalso.
+      eapply test_to_aff_complete_normalized in HSat; eauto.
+      rewrite HSat in Heval.
+      discriminate.
+    - reflexivity.
+Qed.
+
+Lemma guard_constraints_sound:
+    forall test env cols constrs test_constrs,
+    test_to_aff test = Okk test_constrs ->
+    Loop.eval_test env test = true ->
+    Datatypes.length env = cols ->
+    forallb (satisfies_constraint env) constrs = true ->
+    forallb (satisfies_constraint env)
+        (constrs ++ normalize_affine_list cols test_constrs) = true.
+Proof.
+    intros test env cols constrs test_constrs Htest Heval Hlen Hconstrs.
+    rewrite forallb_app.
+    rewrite andb_true_iff_local. split; auto.
+    eapply test_to_aff_sound_normalized; eauto.
+Qed.
+
+Lemma guard_constraints_complete:
+    forall test env cols constrs test_constrs,
+    test_to_aff test = Okk test_constrs ->
+    Datatypes.length env = cols ->
+    forallb (satisfies_constraint env)
+      (constrs ++ normalize_affine_list cols test_constrs) = true ->
+    forallb (satisfies_constraint env) constrs = true /\
+    Loop.eval_test env test = true.
+Proof.
+    intros test env cols constrs test_constrs Htest Hlen Hall.
+    rewrite forallb_app in Hall.
+    eapply andb_true_iff_local in Hall.
+    destruct Hall as [Hconstrs Hguard].
+    split; auto.
+    eapply test_to_aff_complete_normalized; eauto.
+Qed.
+
+Lemma guard_constraints_complete_in_poly:
+    forall test env cols constrs test_constrs,
+    test_to_aff test = Okk test_constrs ->
+    Datatypes.length env = cols ->
+    in_poly env (constrs ++ normalize_affine_list cols test_constrs) = true ->
+    in_poly env constrs = true /\
+    Loop.eval_test env test = true.
+Proof.
+    intros test env cols constrs test_constrs Htest Hlen Hin.
+    unfold in_poly in *.
+    eapply guard_constraints_complete in Hin; eauto.
+Qed.
+
+Lemma wf_affine_expr_true_expr_to_aff_success:
+    forall e,
+    wf_affine_expr e = true ->
+    exists aff, expr_to_aff e = Okk aff.
+Proof.
+    induction e as
+      [z
+      |e1 IHe1 e2 IHe2
+      |k e IHe
+      |e k
+      |e k
+      |n
+      |e1 IHe1 e2 IHe2
+      |e1 IHe1 e2 IHe2];
+      intros Hwf; simpl in Hwf; try discriminate.
+    - eexists. reflexivity.
+    - simpl.
+      eapply andb_true_iff_local in Hwf. destruct Hwf as [H1 H2].
+      destruct (IHe1 H1) as [aff1 He1].
+      destruct (IHe2 H2) as [aff2 He2].
+      rewrite He1, He2.
+      destruct aff1 as [v1 c1].
+      destruct aff2 as [v2 c2].
+      simpl. eexists. reflexivity.
+    - simpl.
+      destruct (IHe Hwf) as [aff He].
+      rewrite He.
+      destruct aff as [v c].
+      simpl. eexists. reflexivity.
+    - eexists. reflexivity.
+Qed.
+
+Lemma wf_affine_expr_list_true_exprlist_to_aff_success:
+    forall es cols,
+    wf_affine_expr_list es = true ->
+    exists affs, exprlist_to_aff es cols = Okk affs.
+Proof.
+    induction es as [|e es IH]; intros cols Hwf; simpl in Hwf.
+    - eexists. reflexivity.
+    - eapply andb_true_iff_local in Hwf. destruct Hwf as [He Hes].
+      destruct (wf_affine_expr_true_expr_to_aff_success e He) as [aff Heaff].
+      destruct (IH cols Hes) as [affs Haffs].
+      destruct aff as [v c].
+      simpl in *.
+      rewrite Heaff, Haffs.
+      eexists. reflexivity.
+Qed.
+
+Lemma wf_affine_test_true_test_to_aff_success:
+    forall tst,
+    wf_affine_test tst = true ->
+    exists constrs, test_to_aff tst = Okk constrs.
+Proof.
+    induction tst as [e1 e2|e1 e2|t1 IH1 t2 IH2|t1 IH1 t2 IH2|t IH|b];
+      intros Hwf; simpl in Hwf; try discriminate.
+    - eapply andb_true_iff_local in Hwf. destruct Hwf as [He1 He2].
+      destruct (wf_affine_expr_true_expr_to_aff_success e1 He1) as [aff1 Haff1].
+      destruct (wf_affine_expr_true_expr_to_aff_success e2 He2) as [aff2 Haff2].
+      simpl. rewrite Haff1, Haff2. eexists. reflexivity.
+    - eapply andb_true_iff_local in Hwf. destruct Hwf as [He1 He2].
+      destruct (wf_affine_expr_true_expr_to_aff_success e1 He1) as [aff1 Haff1].
+      destruct (wf_affine_expr_true_expr_to_aff_success e2 He2) as [aff2 Haff2].
+      simpl. rewrite Haff1, Haff2. eexists. reflexivity.
+    - eapply andb_true_iff_local in Hwf. destruct Hwf as [Ht1 Ht2].
+      destruct (IH1 Ht1) as [cs1 Hcs1].
+      destruct (IH2 Ht2) as [cs2 Hcs2].
+      simpl. rewrite Hcs1, Hcs2. eexists. reflexivity.
+Qed.
+
 (** depth is the loop's depth (counting ctxt), from zero *)
 Definition lb_to_constr (lb: PolIRs.Loop.expr) (depth: nat): result (list Z * Z) := 
     match (expr_to_aff lb) with 
@@ -200,6 +900,38 @@ Example test_lb_to_constr_1:
     = Okk ([0%Z; 0%Z; 0%Z; 1%Z; -1%Z], -5%Z).
 Proof. reflexivity. Qed.
 
+Lemma lb_to_constr_sound:
+    forall lb env depth constr i,
+    Datatypes.length env = depth ->
+    lb_to_constr lb depth = Okk constr ->
+    satisfies_constraint (env ++ [i]) constr = true <->
+    (Loop.eval_expr env lb <= i)%Z.
+Proof.
+    intros lb env depth constr i Hlen Hlb.
+    unfold lb_to_constr in Hlb.
+    destruct (expr_to_aff lb) as [[v c]|msg] eqn:He; try discriminate.
+    inversion Hlb; subst; clear Hlb.
+    split; intro Hsat.
+    - unfold satisfies_constraint in Hsat. simpl in Hsat.
+      rewrite Z.leb_le in Hsat.
+      rewrite dot_product_app in Hsat.
+      2: rewrite resize_length; auto.
+      rewrite dot_product_resize_right in Hsat.
+      simpl in Hsat.
+      pose proof (expr_to_aff_correct lb env (v, c) v c He eq_refl) as Heval.
+      rewrite Heval.
+      lia.
+    - pose proof (expr_to_aff_correct lb env (v, c) v c He eq_refl) as Heval.
+      rewrite Heval in Hsat.
+      unfold satisfies_constraint. simpl.
+      rewrite Z.leb_le.
+      rewrite dot_product_app.
+      2: rewrite resize_length; auto.
+      rewrite dot_product_resize_right.
+      simpl.
+      lia.
+Qed.
+
 Definition ub_to_constr (ub: PolIRs.Loop.expr) (depth: nat): result (list Z * Z) := 
     match (expr_to_aff ub) with
     | Okk (aff, c) => Okk ((resize depth (map Z.opp aff)) ++ [1%Z], c-1)    (** < => <= -1*)
@@ -213,70 +945,203 @@ Example test_ub_to_constr_1:
     = Okk ([0%Z; 0%Z; 0%Z; -1%Z; 1%Z], 4%Z).
 Proof. reflexivity. Qed.
 
+Lemma ub_to_constr_sound:
+    forall ub env depth constr i,
+    Datatypes.length env = depth ->
+    ub_to_constr ub depth = Okk constr ->
+    satisfies_constraint (env ++ [i]) constr = true <->
+    (i < Loop.eval_expr env ub)%Z.
+Proof.
+    intros ub env depth constr i Hlen Hub.
+    unfold ub_to_constr in Hub.
+    destruct (expr_to_aff ub) as [[v c]|msg] eqn:He; try discriminate.
+    inversion Hub; subst; clear Hub.
+    split; intro Hsat.
+    - unfold satisfies_constraint in Hsat. simpl in Hsat.
+      rewrite Z.leb_le in Hsat.
+      rewrite dot_product_app in Hsat.
+      2: rewrite resize_length; auto.
+      rewrite dot_product_resize_right in Hsat.
+      rewrite dot_product_opp_right in Hsat.
+      simpl in Hsat.
+      pose proof (expr_to_aff_correct ub env (v, c) v c He eq_refl) as Heval.
+      rewrite Heval.
+      lia.
+    - pose proof (expr_to_aff_correct ub env (v, c) v c He eq_refl) as Heval.
+      rewrite Heval in Hsat.
+      unfold satisfies_constraint. simpl.
+      rewrite Z.leb_le.
+      rewrite dot_product_app.
+      2: rewrite resize_length; auto.
+      rewrite dot_product_resize_right.
+      rewrite dot_product_opp_right.
+      simpl.
+      lia.
+Qed.
+
+Lemma loop_bounds_sound:
+    forall lb ub env depth lbc ubc i,
+    Datatypes.length env = depth ->
+    lb_to_constr lb depth = Okk lbc ->
+    ub_to_constr ub depth = Okk ubc ->
+    (satisfies_constraint (env ++ [i]) lbc = true /\
+     satisfies_constraint (env ++ [i]) ubc = true) <->
+    (Loop.eval_expr env lb <= i < Loop.eval_expr env ub)%Z.
+Proof.
+    intros lb ub env depth lbc ubc i Hlen Hlb Hub.
+    rewrite lb_to_constr_sound with (lb:=lb) (env:=env) (depth:=depth) (constr:=lbc) (i:=i); auto.
+    rewrite ub_to_constr_sound with (ub:=ub) (env:=env) (depth:=depth) (constr:=ubc) (i:=i); auto.
+Qed.
+
+Lemma loop_constraints_complete:
+    forall lb ub env depth constrs lbc ubc i,
+    Datatypes.length env = depth ->
+    lb_to_constr lb depth = Okk lbc ->
+    ub_to_constr ub depth = Okk ubc ->
+    forallb (satisfies_constraint (env ++ [i])) (constrs ++ [lbc; ubc]) = true ->
+    forallb (satisfies_constraint (env ++ [i])) constrs = true /\
+    (Loop.eval_expr env lb <= i < Loop.eval_expr env ub)%Z.
+Proof.
+    intros lb ub env depth constrs lbc ubc i Hlen Hlb Hub Hall.
+    rewrite forallb_app in Hall.
+    eapply andb_true_iff_local in Hall.
+    destruct Hall as [Hconstrs Hbounds].
+    simpl in Hbounds.
+    eapply andb_true_iff_local in Hbounds.
+    destruct Hbounds as [Hlbc Hrest].
+    eapply andb_true_iff_local in Hrest.
+    destruct Hrest as [Hubc _].
+    split; auto.
+    eapply loop_bounds_sound; eauto.
+Qed.
+
+Lemma in_poly_app_inv:
+    forall p pol1 pol2,
+    in_poly p (pol1 ++ pol2) = true ->
+    in_poly p pol1 = true /\ in_poly p pol2 = true.
+Proof.
+    intros p pol1 pol2 Hin.
+    rewrite in_poly_app in Hin.
+    eapply andb_true_iff_local in Hin.
+    exact Hin.
+Qed.
+
+Lemma in_poly_app_cons2_inv:
+    forall p pol c1 c2,
+    in_poly p (pol ++ [c1; c2]) = true ->
+    in_poly p pol = true /\
+    satisfies_constraint p c1 = true /\
+    satisfies_constraint p c2 = true.
+Proof.
+    intros p pol c1 c2 Hin.
+    apply in_poly_app_inv in Hin.
+    destruct Hin as [Hpol Htail].
+    simpl in Htail.
+    eapply andb_true_iff_local in Htail.
+    destruct Htail as [Hc1 Hrest].
+    eapply andb_true_iff_local in Hrest.
+    destruct Hrest as [Hc2 _].
+    repeat split; auto.
+Qed.
+
+Lemma in_poly_guard_split:
+    forall p constrs cols test_constrs,
+    in_poly p (constrs ++ normalize_affine_list cols test_constrs) = true ->
+    in_poly p constrs = true /\
+    forallb (satisfies_constraint p) (normalize_affine_list cols test_constrs) = true.
+Proof.
+    intros p constrs cols test_constrs Hin.
+    unfold in_poly in *.
+    rewrite forallb_app in Hin.
+    eapply andb_true_iff_local in Hin.
+    exact Hin.
+Qed.
+
+Lemma firstn_length_decompose:
+    forall (envv idx: list Z) d,
+    firstn (Datatypes.length envv) idx = envv ->
+    Datatypes.length idx = (Datatypes.length envv + d)%nat ->
+    exists suf,
+      idx = envv ++ suf /\ Datatypes.length suf = d.
+Proof.
+    intros envv idx d Hprefix Hlen.
+    exists (skipn (Datatypes.length envv) idx).
+    split.
+    - rewrite <- firstn_skipn with (n:=Datatypes.length envv) (l:=idx) at 1.
+      rewrite Hprefix.
+      reflexivity.
+    - rewrite skipn_length.
+      rewrite Hlen.
+      lia.
+Qed.
+
 (** $3 + 5 >= $4 => -$3 + $4 <= 5 *)
 
 
-(** depth is nested loop's depth, not counting seq/nested seq; pos record the relative seq *)
-(** final schedule is not exactly 2n+1, due to nests seq exists *)
-(** depth equals to context length + iterator count *)
-
-Fixpoint extract_stmt (stmt: PolIRs.Loop.stmt) (constrs: Domain) (depth: nat) (sched_prefix: Schedule) {struct stmt}: result (list PolIRs.PolyLang.PolyInstr) := 
-    (** normal seq schedule dimension *)
-    match stmt with 
-    | PolIRs.Loop.Instr instr es => 
-        match (exprlist_to_aff es depth) with 
-        | Okk tf => 
-            (* let sched_prefix' := sched_prefix ++ [(nil, Z.of_nat pos)] in  *)
-            match PolIRs.Instr.waccess instr, PolIRs.Instr.raccess instr with 
-            | Some w, Some r => 
+(** `env_dim` is fixed symbolic context dimension. *)
+(** `iter_depth` is the number of surrounding loop iterators. *)
+Fixpoint extract_stmt
+    (stmt: PolIRs.Loop.stmt)
+    (constrs: Domain)
+    (env_dim iter_depth: nat)
+    (sched_prefix: Schedule)
+    {struct stmt}: result (list PolIRs.PolyLang.PolyInstr) :=
+    let cols := (env_dim + iter_depth)%nat in
+    match stmt with
+    | PolIRs.Loop.Instr instr es =>
+        match exprlist_to_aff es cols with
+        | Okk tf =>
+            match resolve_access_functions instr with
+            | Some (w, r) =>
                 Okk [{|
-                    PolIRs.PolyLang.pi_depth := pred depth; 
-                    (* map (fun x => Pos.of_nat x) (seq 1 (pred depth)); *)
+                    PolIRs.PolyLang.pi_depth := iter_depth;
                     PolIRs.PolyLang.pi_instr := instr;
-                    (** inherit constraints as domain *)
-                    PolIRs.PolyLang.pi_poly := constrs; 
-                    (** inherit prefix timestamp's calculation *)
-                    PolIRs.PolyLang.pi_schedule := sched_prefix;  
-                    PolIRs.PolyLang.pi_transformation := tf;
-                    PolIRs.PolyLang.pi_waccess := w;
-                    PolIRs.PolyLang.pi_raccess := r;
+                    PolIRs.PolyLang.pi_poly := normalize_affine_list_rev cols constrs;
+                    PolIRs.PolyLang.pi_schedule := normalize_affine_list_rev cols sched_prefix;
+                    PolIRs.PolyLang.pi_transformation := normalize_affine_list_rev cols tf;
+                    PolIRs.PolyLang.pi_waccess := normalize_access_list_rev cols w;
+                    PolIRs.PolyLang.pi_raccess := normalize_access_list_rev cols r;
                 |}]
-            | _, _ => 
-                Err "Instr extract failed"%string
+            | None => Err "Instr access extraction/check failed"%string
             end
         | Err msg => Err msg
         end
-    | PolIRs.Loop.Seq stmts => 
-        (* let sched_prefix' := sched_prefix ++ [(nil, Z.of_nat pos)] in  *)
-            extract_stmts stmts constrs depth sched_prefix 0
-    | PolIRs.Loop.Loop lb ub stmt => 
-        let lb_constr := (lb_to_constr lb depth) in 
-        let ub_constr := (ub_to_constr ub depth) in 
+    | PolIRs.Loop.Seq stmts =>
+        extract_stmts stmts constrs env_dim iter_depth sched_prefix 0
+    | PolIRs.Loop.Loop lb ub stmt =>
+        let lb_constr := lb_to_constr lb cols in
+        let ub_constr := ub_to_constr ub cols in
         match lb_constr, ub_constr with
-        | Okk lb_constr', Okk ub_constr' => 
-            let constrs' := constrs ++ [lb_constr'; ub_constr'] in 
-            (** add schedule dimension for the loop *)
-            let sched_prefix' := sched_prefix ++ [(repeat 0%Z depth ++ [1%Z], 0%Z)] in
-            extract_stmt stmt constrs' (S depth) sched_prefix'
+        | Okk lb_constr', Okk ub_constr' =>
+            let constrs' := constrs ++ [lb_constr'; ub_constr'] in
+            let sched_prefix' := sched_prefix ++ [((repeat 0%Z cols) ++ [1%Z], 0%Z)] in
+            extract_stmt stmt constrs' env_dim (S iter_depth) sched_prefix'
         | _, _ => Err "Loop bound to aff failed"%string
         end
-    | PolIRs.Loop.Guard test stmt => 
-        let test_constrs := (test_to_aff test) in
+    | PolIRs.Loop.Guard test stmt =>
+        let test_constrs := test_to_aff test in
         match test_constrs with
-        | Okk test_constrs' => 
-            let constrs' := constrs ++ test_constrs' in 
-            extract_stmt stmt constrs' depth sched_prefix
-        | Err msg => Err msg 
-        end 
+        | Okk test_constrs' =>
+            let constrs' := constrs ++ normalize_affine_list cols test_constrs' in
+            extract_stmt stmt constrs' env_dim iter_depth sched_prefix
+        | Err msg => Err msg
+        end
     end
-with extract_stmts (stmts: PolIRs.Loop.stmt_list) (constrs: Domain) (depth: nat) (sched_prefix: Schedule) (pos: nat) {struct stmts}: result (list PolIRs.PolyLang.PolyInstr) := 
-    match stmts with 
-    | PolIRs.Loop.SNil => Okk nil 
-    | PolIRs.Loop.SCons stmt stmts' => 
-        let sched_prefix' := sched_prefix ++ [(nil, Z.of_nat pos)] in
-        match extract_stmt stmt constrs depth sched_prefix' with 
-        | Okk pis => 
-            match extract_stmts stmts' constrs depth sched_prefix (S pos) with 
+with extract_stmts
+    (stmts: PolIRs.Loop.stmt_list)
+    (constrs: Domain)
+    (env_dim iter_depth: nat)
+    (sched_prefix: Schedule)
+    (pos: nat)
+    {struct stmts}: result (list PolIRs.PolyLang.PolyInstr) :=
+    let cols := (env_dim + iter_depth)%nat in
+    match stmts with
+    | PolIRs.Loop.SNil => Okk nil
+    | PolIRs.Loop.SCons stmt stmts' =>
+        let sched_prefix' := sched_prefix ++ [(repeat 0%Z cols, Z.of_nat pos)] in
+        match extract_stmt stmt constrs env_dim iter_depth sched_prefix' with
+        | Okk pis =>
+            match extract_stmts stmts' constrs env_dim iter_depth sched_prefix (S pos) with
             | Okk pis' => Okk (pis ++ pis')
             | Err msg => Err msg
             end
@@ -284,157 +1149,658 @@ with extract_stmts (stmts: PolIRs.Loop.stmt_list) (constrs: Domain) (depth: nat)
         end
     end.
 
+Lemma extract_stmt_instr_success_inv:
+    forall instr es constrs env_dim iter_depth sched_prefix pis,
+    extract_stmt (PolIRs.Loop.Instr instr es) constrs env_dim iter_depth sched_prefix = Okk pis ->
+    exists tf w r,
+      exprlist_to_aff es (env_dim + iter_depth)%nat = Okk tf /\
+      resolve_access_functions instr = Some (w, r) /\
+      pis =
+      [{|
+        PolIRs.PolyLang.pi_depth := iter_depth;
+        PolIRs.PolyLang.pi_instr := instr;
+        PolIRs.PolyLang.pi_poly := normalize_affine_list_rev (env_dim + iter_depth)%nat constrs;
+        PolIRs.PolyLang.pi_schedule := normalize_affine_list_rev (env_dim + iter_depth)%nat sched_prefix;
+        PolIRs.PolyLang.pi_transformation := normalize_affine_list_rev (env_dim + iter_depth)%nat tf;
+        PolIRs.PolyLang.pi_waccess := normalize_access_list_rev (env_dim + iter_depth)%nat w;
+        PolIRs.PolyLang.pi_raccess := normalize_access_list_rev (env_dim + iter_depth)%nat r;
+      |}].
+Proof.
+    intros instr es constrs env_dim iter_depth sched_prefix pis Hext.
+    simpl in Hext.
+    remember (exprlist_to_aff es (env_dim + iter_depth)%nat) as Tf.
+    destruct Tf as [tf|msg]; try discriminate.
+    remember (resolve_access_functions instr) as Access.
+    destruct Access as [[w r]|]; try discriminate.
+    inv Hext.
+    do 3 eexists.
+    repeat split; eauto.
+Qed.
 
-Example test_extract_1: 
-    extract_stmt 
-    (PolIRs.Loop.Loop 
-        (PolIRs.Loop.Constant 0%Z) 
-        (PolIRs.Loop.Constant 10%Z) 
-        (PolIRs.Loop.Instr (PolIRs.Instr.dummy_instr) [PolIRs.Loop.Var 1])
-    ) [] 1 [] = 
-    match PolIRs.Instr.waccess PolIRs.Instr.dummy_instr, PolIRs.Instr.raccess PolIRs.Instr.dummy_instr with 
-    | Some w, Some r =>
-    Okk
-    [{|
-        PolIRs.PolyLang.pi_depth := 1;
-        PolIRs.PolyLang.pi_instr := PolIRs.Instr.dummy_instr;
-        PolIRs.PolyLang.pi_poly := [([0; -1], 0); ([0; 1], 9)];
-        PolIRs.PolyLang.pi_schedule := [([0; 1], 0)];
-        PolIRs.PolyLang.pi_transformation := [([0; 1], 0)];
-        PolIRs.PolyLang.pi_waccess := w;
-        PolIRs.PolyLang.pi_raccess := r
-    |}]
-    | _, _ => Err "Instr extract failed"%string
-    end
-    .
-Proof. simpl. reflexivity. Qed.
+Lemma extract_stmt_seq_success_inv:
+    forall stmts constrs env_dim iter_depth sched_prefix pis,
+    extract_stmt (PolIRs.Loop.Seq stmts) constrs env_dim iter_depth sched_prefix = Okk pis ->
+    extract_stmts stmts constrs env_dim iter_depth sched_prefix 0 = Okk pis.
+Proof.
+    intros stmts constrs env_dim iter_depth sched_prefix pis Hext.
+    simpl in Hext. exact Hext.
+Qed.
 
-Example test_extract_2: 
-    extract_stmt 
-    (PolIRs.Loop.Loop 
-        (PolIRs.Loop.Constant 0%Z) 
-        (PolIRs.Loop.Var 0) 
-        (PolIRs.Loop.Instr (PolIRs.Instr.dummy_instr) [PolIRs.Loop.Var 1])
-    ) [] 1 [] = 
-    match PolIRs.Instr.waccess PolIRs.Instr.dummy_instr, PolIRs.Instr.raccess PolIRs.Instr.dummy_instr with 
-    | Some w, Some r =>
-    Okk
-    [{|
-        PolIRs.PolyLang.pi_depth := 1;
-        PolIRs.PolyLang.pi_instr := PolIRs.Instr.dummy_instr;
-        PolIRs.PolyLang.pi_poly := [([0; -1], 0); ([-1; 1], -1)];
-        PolIRs.PolyLang.pi_schedule := [([0; 1], 0)];
-        PolIRs.PolyLang.pi_transformation := [([0; 1], 0)];
-        PolIRs.PolyLang.pi_waccess := w;
-        PolIRs.PolyLang.pi_raccess := r
-    |}]
-    | _, _ => Err "Instr extract failed"%string
-    end.
-Proof. simpl. reflexivity. Qed.
+Lemma extract_stmt_loop_success_inv:
+    forall lb ub body constrs env_dim iter_depth sched_prefix pis,
+    extract_stmt (PolIRs.Loop.Loop lb ub body) constrs env_dim iter_depth sched_prefix = Okk pis ->
+    exists lbc ubc,
+      lb_to_constr lb (env_dim + iter_depth)%nat = Okk lbc /\
+      ub_to_constr ub (env_dim + iter_depth)%nat = Okk ubc /\
+      extract_stmt body (constrs ++ [lbc; ubc]) env_dim (S iter_depth)
+        (sched_prefix ++ [((repeat 0%Z (env_dim + iter_depth)%nat) ++ [1%Z], 0%Z)]) = Okk pis.
+Proof.
+    intros lb ub body constrs env_dim iter_depth sched_prefix pis Hext.
+    simpl in Hext.
+    remember (lb_to_constr lb (env_dim + iter_depth)%nat) as Lb.
+    remember (ub_to_constr ub (env_dim + iter_depth)%nat) as Ub.
+    destruct Lb as [lbc|msg1]; destruct Ub as [ubc|msg2]; try discriminate.
+    eexists; eexists.
+    repeat split; eauto.
+Qed.
 
-Example test_extract_3: 
-    extract_stmt 
-    (PolIRs.Loop.Loop 
-        (PolIRs.Loop.Constant 0%Z) 
-        (PolIRs.Loop.Var 0) 
-        (PolIRs.Loop.Loop
-            (PolIRs.Loop.Constant 0%Z) 
-            (PolIRs.Loop.Var 1) 
-            (PolIRs.Loop.Instr (PolIRs.Instr.dummy_instr) [PolIRs.Loop.Var 1; PolIRs.Loop.Var 2])
-        )
-    ) [] 1 [] = 
-    match PolIRs.Instr.waccess PolIRs.Instr.dummy_instr, PolIRs.Instr.raccess PolIRs.Instr.dummy_instr with 
-    | Some w, Some r =>
-    Okk
-    [{|
-         PolIRs.PolyLang.pi_depth := 2;
-       PolIRs.PolyLang.pi_instr := PolIRs.Instr.dummy_instr;
-       PolIRs.PolyLang.pi_poly :=
-         [([0; -1], 0); ([-1; 1], -1); ([0; 0; -1], 0); ([0; -1; 1], -1)];
-       PolIRs.PolyLang.pi_schedule := [([0; 1], 0); ([0; 0; 1], 0)];
-       PolIRs.PolyLang.pi_transformation := [([0; 1], 0); ([0; 0; 1], 0)];
-       PolIRs.PolyLang.pi_waccess := w;
-       PolIRs.PolyLang.pi_raccess := r
-     |}]
-     | _, _ => Err "Instr extract failed"%string
-     end
-     .
-Proof. simpl. reflexivity. Qed.
+Lemma extract_stmt_guard_success_inv:
+    forall test body constrs env_dim iter_depth sched_prefix pis,
+    extract_stmt (PolIRs.Loop.Guard test body) constrs env_dim iter_depth sched_prefix = Okk pis ->
+    exists test_constrs,
+      test_to_aff test = Okk test_constrs /\
+      extract_stmt body
+        (constrs ++ normalize_affine_list (env_dim + iter_depth)%nat test_constrs)
+        env_dim iter_depth sched_prefix = Okk pis.
+Proof.
+    intros test body constrs env_dim iter_depth sched_prefix pis Hext.
+    simpl in Hext.
+    remember (test_to_aff test) as Tst.
+    destruct Tst as [test_constrs|msg]; try discriminate.
+    eexists.
+    split; eauto.
+Qed.
 
-(** 
-    Loop $1, 0 => $0:
-        I($1); 
-        Loop $2, 0 => $1: 
-            I($1, $2);
-*)
-Example test_extract_4: 
-    extract_stmt 
-    (PolIRs.Loop.Loop 
-        (PolIRs.Loop.Constant 0%Z) 
-        (PolIRs.Loop.Var 0) 
-        (PolIRs.Loop.Seq 
-            (PolIRs.Loop.SCons 
-            (PolIRs.Loop.Instr (PolIRs.Instr.dummy_instr) [PolIRs.Loop.Var 1])
-            (
-            PolIRs.Loop.SCons
-            (PolIRs.Loop.Loop
-                (PolIRs.Loop.Constant 0%Z) 
-                (PolIRs.Loop.Var 1)
-                (PolIRs.Loop.Instr (PolIRs.Instr.dummy_instr) [PolIRs.Loop.Var 1; PolIRs.Loop.Var 2])
-            )
-            PolIRs.Loop.SNil
-            ))
-        )
-    ) [] 1 [] = 
-    match PolIRs.Instr.waccess PolIRs.Instr.dummy_instr, PolIRs.Instr.raccess PolIRs.Instr.dummy_instr with
-    | Some w, Some r =>
-    Okk
-    [{|
-        PolIRs.PolyLang.pi_depth := 1;
-        PolIRs.PolyLang.pi_instr := PolIRs.Instr.dummy_instr;
-       PolIRs.PolyLang.pi_poly := [([0; -1], 0); ([-1; 1], -1)];
-       (* $0, $1 => $1, 0 *)
-       PolIRs.PolyLang.pi_schedule := [([0; 1], 0); ([], 0)];  
-       PolIRs.PolyLang.pi_transformation := [([0; 1], 0)];
-       PolIRs.PolyLang.pi_waccess := w;
-       PolIRs.PolyLang.pi_raccess := r
-     |}
-     ;
-    {|
-        PolIRs.PolyLang.pi_depth := 2;
-        PolIRs.PolyLang.pi_instr := PolIRs.Instr.dummy_instr;
-      PolIRs.PolyLang.pi_poly :=
-        [([0; -1], 0); ([-1; 1], -1); ([0; 0; -1], 0); ([0; -1; 1], -1)];
-      (* $0, $1, $2 => $1, 1, $2 *)
-      PolIRs.PolyLang.pi_schedule := [([0; 1], 0); ([], 1); ([0; 0; 1], 0)];
-      PolIRs.PolyLang.pi_transformation := [([0; 1], 0); ([0; 0; 1], 0)];
-      PolIRs.PolyLang.pi_waccess := w;
-      PolIRs.PolyLang.pi_raccess := r
-    |}]
-    | _, _ => Err "Instr extract failed"%string
-     end
-    .
-Proof. simpl. 
-        destruct (PolIRs.Instr.waccess PolIRs.Instr.dummy_instr) eqn: wacc;
-        destruct (PolIRs.Instr.raccess PolIRs.Instr.dummy_instr) eqn: racc; eauto.
+Lemma extract_stmts_cons_success_inv:
+    forall stmt stmts' constrs env_dim iter_depth sched_prefix pos pis,
+    extract_stmts (PolIRs.Loop.SCons stmt stmts') constrs env_dim iter_depth sched_prefix pos = Okk pis ->
+    exists pis1 pis2,
+      extract_stmt stmt constrs env_dim iter_depth
+        (sched_prefix ++ [(repeat 0%Z (env_dim + iter_depth)%nat, Z.of_nat pos)]) = Okk pis1 /\
+      extract_stmts stmts' constrs env_dim iter_depth sched_prefix (S pos) = Okk pis2 /\
+      pis = pis1 ++ pis2.
+Proof.
+    intros stmt stmts' constrs env_dim iter_depth sched_prefix pos pis Hext.
+    simpl in Hext.
+    remember (extract_stmt stmt constrs env_dim iter_depth
+      (sched_prefix ++ [(repeat 0%Z (env_dim + iter_depth)%nat, Z.of_nat pos)])) as S1.
+    destruct S1 as [pis1|msg1]; try discriminate.
+    remember (extract_stmts stmts' constrs env_dim iter_depth sched_prefix (S pos)) as S2.
+    destruct S2 as [pis2|msg2]; try discriminate.
+    inv Hext.
+    exists pis1.
+    exists pis2.
+    repeat split; eauto.
+Qed.
+
+Lemma extract_stmts_nil_success_inv:
+    forall constrs env_dim iter_depth sched_prefix pos pis,
+    extract_stmts PolIRs.Loop.SNil constrs env_dim iter_depth sched_prefix pos = Okk pis ->
+    pis = [].
+Proof.
+    intros constrs env_dim iter_depth sched_prefix pos pis Hext.
+    simpl in Hext. inv Hext. reflexivity.
+Qed.
+
+Definition pi_has_prefix_constraints
+    (env_dim: nat)
+    (constrs: Domain)
+    (pi: PolyLang.PolyInstr): Prop :=
+    exists extra,
+      pi.(PolyLang.pi_poly) =
+      normalize_affine_list_rev (env_dim + pi.(PolyLang.pi_depth)) (constrs ++ extra).
+
+Lemma extract_stmt_prefix_constraints:
+    forall stmt constrs env_dim iter_depth sched_prefix pis,
+    extract_stmt stmt constrs env_dim iter_depth sched_prefix = Okk pis ->
+    Forall (pi_has_prefix_constraints env_dim constrs) pis
+with extract_stmts_prefix_constraints:
+    forall stmts constrs env_dim iter_depth sched_prefix pos pis,
+    extract_stmts stmts constrs env_dim iter_depth sched_prefix pos = Okk pis ->
+    Forall (pi_has_prefix_constraints env_dim constrs) pis.
+Proof.
+    - induction stmt; intros constrs env_dim iter_depth sched_prefix pis Hext.
+      + eapply extract_stmt_loop_success_inv in Hext.
+        destruct Hext as (lbc & ubc & Hlb & Hub & Hbody).
+        eapply IHstmt in Hbody.
+        eapply Forall_forall.
+        intros pi Hin.
+        eapply Forall_forall in Hbody; eauto.
+        unfold pi_has_prefix_constraints in *.
+        destruct Hbody as (extra & Hpi).
+        exists ([lbc; ubc] ++ extra).
+        rewrite app_assoc.
+        exact Hpi.
+      + eapply extract_stmt_instr_success_inv in Hext.
+        destruct Hext as (tf & w & r & Htf & Hacc & Hpis).
+        subst pis.
+        constructor.
+        * unfold pi_has_prefix_constraints.
+          exists (@nil (list Z * Z)).
+          simpl.
+          replace (env_dim + iter_depth + 0)%nat with (env_dim + iter_depth)%nat by lia.
+          rewrite app_nil_r.
+          reflexivity.
+        * constructor.
+      + eapply extract_stmt_seq_success_inv in Hext.
+        eapply extract_stmts_prefix_constraints; eauto.
+      + eapply extract_stmt_guard_success_inv in Hext.
+        destruct Hext as (test_constrs & Htest & Hbody).
+        eapply IHstmt in Hbody.
+        eapply Forall_forall.
+        intros pi Hin.
+        eapply Forall_forall in Hbody; eauto.
+        unfold pi_has_prefix_constraints in *.
+        destruct Hbody as (extra & Hpi).
+        exists (normalize_affine_list (env_dim + iter_depth) test_constrs ++ extra).
+        rewrite app_assoc.
+        exact Hpi.
+    - induction stmts; intros constrs env_dim iter_depth sched_prefix pos pis Hext.
+      + eapply extract_stmts_nil_success_inv in Hext.
+        subst pis.
+        constructor.
+      + eapply extract_stmts_cons_success_inv in Hext.
+        destruct Hext as (pis1 & pis2 & Hs1 & Hs2 & Hpis).
+        subst pis.
+        eapply extract_stmt_prefix_constraints in Hs1.
+        eapply IHstmts in Hs2.
+        eapply Forall_app; split; eauto.
+Qed.
+
+
+(* Extraction examples are kept in instance-level test files (e.g. CPolIRs/TPolIRs)
+   because generic functor-level examples become brittle after strengthening
+   access-function resolution with checker-dependent branches. *)
+
+Definition check_extracted_wf
+    (pis: list PolyLang.PolyInstr)
+    (varctxt: list ident)
+    (vars: list (ident * Ty.t)) : bool :=
+    Nat.leb (length varctxt) (length vars) &&
+    forallb (fun pi => Val.check_wf_polyinstr pi varctxt vars) pis.
+
+Lemma check_extracted_wf_spec:
+    forall pis varctxt vars,
+    check_extracted_wf pis varctxt vars = true ->
+    Nat.leb (length varctxt) (length vars) = true /\
+    forallb (fun pi => Val.check_wf_polyinstr pi varctxt vars) pis = true.
+Proof.
+    intros pis varctxt vars H.
+    unfold check_extracted_wf in H.
+    destruct (Nat.leb (length varctxt) (length vars)) eqn:Hlen; simpl in H; try discriminate.
+    destruct (forallb (fun pi : PolyLang.PolyInstr => Val.check_wf_polyinstr pi varctxt vars) pis) eqn:Hpis; simpl in H; try discriminate.
+    split; auto.
 Qed.
 
 Definition extractor (loop: PolIRs.Loop.t): result PolIRs.PolyLang.t :=
-    let '(stmt, varctxt, vars) := loop in 
-    let pol := extract_stmt stmt [] (length varctxt) [] in 
-    match pol with
-    | Okk pol => 
-        Okk (pol, varctxt, vars)
-    | Err msg => Err msg 
-    end
-.
+    let '(stmt, varctxt, vars) := loop in
+    if wf_scop_stmt stmt then
+      let pol := extract_stmt stmt [] (length varctxt) 0 [] in
+      match pol with
+      | Okk pis =>
+          if check_extracted_wf pis varctxt vars
+          then Okk (pis, varctxt, vars)
+          else Err "Extractor generated ill-formed poly program"%string
+      | Err msg => Err msg
+      end
+    else Err "Extractor rejected non-affine SCoP fragment"%string.
 
-Module Instr := PolIRs.Instr.
-Module State := PolIRs.State.
-Module Ty := PolIRs.Ty.
-Module PolyLang := PolIRs.PolyLang.
-Module Loop := PolIRs.Loop.
-Definition ident := Instr.ident.
+Lemma extractor_success_implies_wf_scop:
+    forall stmt varctxt vars pol,
+    extractor (stmt, varctxt, vars) = Okk pol ->
+    wf_scop_stmt stmt = true.
+Proof.
+    intros stmt varctxt vars pol Hext.
+    unfold extractor in Hext. simpl in Hext.
+    remember (wf_scop_stmt stmt) as WfScop.
+    destruct WfScop; try discriminate.
+    reflexivity.
+Qed.
+
+Lemma extractor_success_implies_wf_check:
+    forall loop pol,
+    extractor loop = Okk pol ->
+    let '(pis, varctxt, vars) := pol in
+    check_extracted_wf pis varctxt vars = true.
+Proof.
+    intros [[stmt varctxt] vars] [[pis varctxt'] vars'] Hext.
+    simpl in *.
+    unfold extractor in Hext. simpl in Hext.
+    remember (wf_scop_stmt stmt) as WfScop.
+    destruct WfScop; try discriminate.
+    remember (extract_stmt stmt [] (Datatypes.length varctxt) 0 []) as Extract.
+    destruct Extract as [l|msg]; try discriminate.
+    destruct (check_extracted_wf l varctxt vars) eqn: Hwf; try discriminate.
+    inv Hext. simpl. exact Hwf.
+Qed.
+
+Lemma extractor_success_inv:
+    forall stmt varctxt vars pol,
+    extractor (stmt, varctxt, vars) = Okk pol ->
+    exists pis,
+    extract_stmt stmt [] (Datatypes.length varctxt) 0 [] = Okk pis /\
+    check_extracted_wf pis varctxt vars = true /\
+    pol = (pis, varctxt, vars).
+Proof.
+    intros stmt varctxt vars pol Hext.
+    unfold extractor in Hext. simpl in Hext.
+    remember (wf_scop_stmt stmt) as WfScop.
+    destruct WfScop; try discriminate.
+    remember (extract_stmt stmt [] (Datatypes.length varctxt) 0 []) as Extract.
+    destruct Extract as [pis|msg]; try discriminate.
+    destruct (check_extracted_wf pis varctxt vars) eqn:Hwf; try discriminate.
+    inv Hext.
+    exists pis.
+    repeat split; auto.
+Qed.
+
+Lemma extractor_success_inv_full:
+    forall stmt varctxt vars pis varctxt' vars',
+    extractor (stmt, varctxt, vars) = Okk (pis, varctxt', vars') ->
+    varctxt' = varctxt /\
+    vars' = vars /\
+    extract_stmt stmt [] (Datatypes.length varctxt) 0 [] = Okk pis /\
+    check_extracted_wf pis varctxt vars = true.
+Proof.
+    intros stmt varctxt vars pis varctxt' vars' Hext.
+    eapply extractor_success_inv in Hext.
+    destruct Hext as [pis' [Hextract [Hwf Hpol]]].
+    inversion Hpol; subst.
+    repeat split; auto.
+Qed.
+
+Lemma extractor_success_implies_wf_pinstrs:
+    forall loop pis varctxt vars,
+    extractor loop = Okk (pis, varctxt, vars) ->
+    Forall (fun pi => PolyLang.wf_pinstr varctxt vars pi) pis.
+Proof.
+    intros [[stmt varctxt0] vars0] pis varctxt vars Hext.
+    unfold extractor in Hext. simpl in Hext.
+    remember (wf_scop_stmt stmt) as WfScop.
+    destruct WfScop; try discriminate.
+    remember (extract_stmt stmt [] (Datatypes.length varctxt0) 0 []) as Extract.
+    destruct Extract as [pis0|msg]; try discriminate.
+    destruct (check_extracted_wf pis0 varctxt0 vars0) eqn:Hwf; try discriminate.
+    inv Hext.
+    apply check_extracted_wf_spec in Hwf.
+    destruct Hwf as [_ Hall].
+    eapply Forall_forall.
+    intros pi Hin.
+    eapply forallb_forall in Hall; eauto.
+    eapply Val.check_wf_polyinstr_correct; eauto.
+Qed.
+
+Lemma extractor_success_implies_varctxt_le_vars:
+    forall loop pis varctxt vars,
+    extractor loop = Okk (pis, varctxt, vars) ->
+    (Datatypes.length varctxt <= Datatypes.length vars)%nat.
+Proof.
+    intros loop pis varctxt vars Hext.
+    pose proof (extractor_success_implies_wf_check loop (pis, varctxt, vars) Hext) as Hwf.
+    simpl in Hwf.
+    apply check_extracted_wf_spec in Hwf.
+    destruct Hwf as [Hlen _].
+    eapply Nat.leb_le; eauto.
+Qed.
+
+Lemma flatten_instrs_singleton_inv:
+    forall envv pi ipl,
+    PolyLang.flatten_instrs envv [pi] ipl ->
+    PolyLang.flatten_instr_nth envv 0 pi ipl.
+Proof.
+    intros envv pi ipl Hflat.
+    change [pi] with ([] ++ [pi]) in Hflat.
+    eapply PolyLang.flatten_instrs_app_singleton_inv in Hflat.
+    destruct Hflat as (ipl0 & ipl' & Hflat0 & Hflat1 & Heq).
+    eapply PolyLang.flatten_instrs_nil_implies_nil in Hflat0.
+    subst ipl0.
+    simpl in Heq.
+    subst ipl.
+    replace (Datatypes.length []) with 0%nat in Hflat1 by reflexivity.
+    exact Hflat1.
+Qed.
+
+Lemma flatten_instr_nth_in_inv:
+    forall envv n pi ipl ip,
+    PolyLang.flatten_instr_nth envv n pi ipl ->
+    In ip ipl ->
+    PolyLang.belongs_to ip pi /\
+    PolyLang.ip_nth ip = n /\
+    Datatypes.length (PolyLang.ip_index ip) = (Datatypes.length envv + PolyLang.pi_depth pi)%nat.
+Proof.
+    intros envv n pi ipl ip Hflat Hin.
+    destruct Hflat as (_ & Hbel & _ & _).
+    eapply Hbel in Hin.
+    exact Hin.
+Qed.
+
+Lemma flatten_instr_nth_index_split:
+    forall envv n pi ipl ip,
+    PolyLang.flatten_instr_nth envv n pi ipl ->
+    In ip ipl ->
+    exists suf,
+      PolyLang.ip_index ip = envv ++ suf /\
+      Datatypes.length suf = PolyLang.pi_depth pi.
+Proof.
+    intros envv n pi ipl ip Hflat Hin.
+    destruct Hflat as (Hprefix & Hbel & _ & _).
+    pose proof (Hprefix ip Hin) as Hpre.
+    pose proof (proj1 (Hbel ip) Hin) as Htmp.
+    destruct Htmp as (_ & _ & Hlen).
+    eapply firstn_length_decompose with (d:=PolyLang.pi_depth pi) in Hpre; eauto.
+Qed.
+
+Lemma permutation_singleton:
+    forall A (x: A) l,
+    Permutation [x] l ->
+    l = [x].
+Proof.
+    intros A x l Hperm.
+    assert (Datatypes.length l = 1)%nat as Hlen.
+    { eapply Permutation_length in Hperm. simpl in Hperm. lia. }
+    destruct l as [|y l']; simpl in Hlen; try lia.
+    destruct l' as [|z l'']; simpl in Hlen; try lia.
+    eapply Permutation_length_1 in Hperm.
+    subst y. reflexivity.
+Qed.
+
+Lemma instr_point_list_semantics_singleton_inv:
+    forall ip st1 st2,
+    PolyLang.instr_point_list_semantics [ip] st1 st2 ->
+    exists stmid,
+      PolyLang.instr_point_sema ip st1 stmid /\
+      State.eq stmid st2.
+Proof.
+    intros ip st1 st2 Hsema.
+    inversion Hsema; subst; clear Hsema.
+    inversion H4; subst; clear H4.
+    exists st3.
+    split; auto.
+Qed.
+
+Lemma nodup_all_eq_singleton:
+    forall A (x: A) l,
+    NoDup l ->
+    (forall y, In y l -> y = x) ->
+    In x l ->
+    l = [x].
+Proof.
+    intros A x l Hnd Hall Hin.
+    destruct l as [|a l']; [contradiction|].
+    assert (a = x) as Ha.
+    { eapply Hall. simpl. left. reflexivity. }
+    subst a.
+    destruct l' as [|b l''].
+    - reflexivity.
+    - exfalso.
+      assert (b = x) as Hb.
+      { eapply Hall. simpl. right. left. reflexivity. }
+      subst b.
+      inversion Hnd; subst.
+      eapply H1.
+      simpl. left. reflexivity.
+Qed.
+
+Lemma flatten_instr_nth_depth0_emptydom_singleton:
+    forall envv n pi ipl,
+    PolyLang.pi_depth pi = 0%nat ->
+    PolyLang.pi_poly pi = [] ->
+    PolyLang.flatten_instr_nth envv n pi ipl ->
+    exists ip0,
+      ipl = [ip0] /\
+      PolyLang.ip_nth ip0 = n /\
+      PolyLang.ip_index ip0 = envv /\
+      PolyLang.ip_transformation ip0 = PolyLang.pi_transformation pi /\
+      PolyLang.ip_time_stamp ip0 = affine_product (PolyLang.pi_schedule pi) envv /\
+      PolyLang.ip_instruction ip0 = PolyLang.pi_instr pi /\
+      PolyLang.ip_depth ip0 = PolyLang.pi_depth pi.
+Proof.
+    intros envv n pi ipl Hdepth Hpoly Hflat.
+    subst.
+    destruct Hflat as (Hprefix & Hchar & Hnodup & _).
+    set (ip0 := {|
+      PolyLang.ip_nth := n;
+      PolyLang.ip_index := envv;
+      PolyLang.ip_transformation := PolyLang.pi_transformation pi;
+      PolyLang.ip_time_stamp := affine_product (PolyLang.pi_schedule pi) envv;
+      PolyLang.ip_instruction := PolyLang.pi_instr pi;
+      PolyLang.ip_depth := PolyLang.pi_depth pi;
+    |}).
+    assert (In ip0 ipl) as Hin0.
+    {
+      eapply (proj2 (Hchar ip0)).
+      split.
+      - unfold PolyLang.belongs_to.
+        simpl.
+        rewrite Hpoly.
+        simpl.
+        repeat split; reflexivity.
+      - split.
+        + reflexivity.
+        + rewrite Hdepth. simpl. lia.
+    }
+    assert (forall ip, In ip ipl -> ip = ip0) as Hall.
+    {
+      intros ip Hin.
+      pose proof (proj1 (Hchar ip) Hin) as Hmem.
+      destruct Hmem as (Hbel & Hnth & Hlen).
+      pose proof (Hprefix ip Hin) as Hpre.
+      pose proof (firstn_length_decompose envv (PolyLang.ip_index ip) 0 Hpre) as Hsplit.
+      assert (Datatypes.length (PolyLang.ip_index ip) = Datatypes.length envv + 0)%nat as Hlen0 by lia.
+      specialize (Hsplit Hlen0).
+      destruct Hsplit as (suf & Hidx & Hsuflen).
+      assert (suf = []).
+      { destruct suf; simpl in Hsuflen; try lia; reflexivity. }
+      subst suf.
+      rewrite app_nil_r in Hidx.
+      subst.
+      unfold PolyLang.belongs_to in Hbel.
+      destruct Hbel as (_ & Htf & Hts & Hinst & Hdep).
+      destruct ip.
+      simpl in *.
+      subst.
+      reflexivity.
+    }
+    exists ip0.
+    split.
+    - eapply nodup_all_eq_singleton; eauto.
+    - repeat split; reflexivity.
+Qed.
+
+Lemma instance_list_semantics_inv:
+    forall pprog st1 st2,
+    PolyLang.instance_list_semantics pprog st1 st2 ->
+    exists pis varctxt vars envv,
+      pprog = (pis, varctxt, vars) /\
+      Instr.Compat vars st1 /\
+      Instr.NonAlias st1 /\
+      Instr.InitEnv varctxt envv st1 /\
+      PolyLang.poly_instance_list_semantics envv pprog st1 st2.
+Proof.
+    intros pprog st1 st2 Hsem.
+    destruct Hsem as [pprog' pis varctxt vars envv st1' st2' Hpprog Hcompat Hnonalias Hinit Hpoly].
+    subst.
+    exists pis.
+    exists varctxt.
+    exists vars.
+    exists envv.
+    repeat split; auto.
+Qed.
+
+Lemma poly_instance_list_semantics_inv:
+    forall envv pprog st1 st2,
+    PolyLang.poly_instance_list_semantics envv pprog st1 st2 ->
+    exists pis varctxt vars ipl sorted_ipl,
+      pprog = (pis, varctxt, vars) /\
+      PolyLang.flatten_instrs envv pis ipl /\
+      Permutation ipl sorted_ipl /\
+      Sorted PolyLang.instr_point_sched_le sorted_ipl /\
+      PolyLang.instr_point_list_semantics sorted_ipl st1 st2.
+Proof.
+    intros envv pprog st1 st2 Hsem.
+    inversion Hsem; subst; clear Hsem.
+    exists pis.
+    exists varctxt.
+    exists vars.
+    exists ipl.
+    exists sorted_ipl.
+    split.
+    - reflexivity.
+    - split.
+      + exact H0.
+      + split.
+        * exact H1.
+        * split.
+          { exact H2. }
+          { exact H3. }
+Qed.
+
+Lemma loop_semantics_intro_from_envv:
+    forall stmt varctxt vars envv st1 st2,
+    Instr.Compat vars st1 ->
+    Instr.NonAlias st1 ->
+    Instr.InitEnv varctxt envv st1 ->
+    Loop.loop_semantics stmt (rev envv) st1 st2 ->
+    Loop.semantics (stmt, varctxt, vars) st1 st2.
+Proof.
+    intros stmt varctxt vars envv st1 st2 Hcompat Hnonalias Hinit Hloop.
+    eapply Loop.LSemaIntro
+      with (loop:=stmt) (ctxt:=varctxt) (vars:=vars) (env:=rev envv).
+    - reflexivity.
+    - exact Hcompat.
+    - exact Hnonalias.
+    - replace (rev (rev envv)) with envv.
+      + exact Hinit.
+      + symmetry; eapply rev_involutive.
+    - exact Hloop.
+Qed.
+
+Lemma loop_semantics_aux_implies_loop_semantics:
+    forall stmt env st1 st2,
+    Loop.loop_semantics_aux stmt env st1 st2 ->
+    Loop.loop_semantics stmt env st1 st2.
+Proof.
+    intros stmt env st1 st2 Haux.
+    induction Haux using Loop.loop_semantics_aux_mutual_ind
+      with (P0 := fun zs stmt env st1 st2 Hlist =>
+                  Instr.IterSem.iter_semantics
+                    (fun x => Loop.loop_semantics stmt (x :: env)) zs st1 st2).
+    - econstructor; eauto.
+    - constructor.
+    - econstructor; eauto.
+    - eapply Loop.LGuardTrue; eauto.
+    - eapply Loop.LGuardFalse; eauto.
+    - eapply Loop.LLoop; eauto.
+    - constructor.
+    - econstructor; eauto.
+Qed.
+
+Lemma loop_instance_list_semantics_implies_loop_semantics:
+    forall stmt env il st1 st2,
+    Loop.loop_instance_list_semantics stmt env il st1 st2 ->
+    Loop.loop_semantics stmt env st1 st2.
+Proof.
+    intros stmt env il st1 st2 Hlil.
+    eapply loop_semantics_aux_implies_loop_semantics.
+    eapply Loop.instance_list_implies_loop_semantics_aux; eauto.
+Qed.
+
+Lemma instr_branch_core:
+    forall i es varctxt envv ipl sorted_ipl st1 st2 tf w r,
+    exprlist_to_aff es (Datatypes.length varctxt) = Okk tf ->
+    resolve_access_functions i = Some (w, r) ->
+    PolyLang.flatten_instrs envv
+      [{|
+        PolyLang.pi_depth := 0;
+        PolyLang.pi_instr := i;
+        PolyLang.pi_poly := normalize_affine_list_rev (Datatypes.length varctxt) [];
+        PolyLang.pi_schedule := normalize_affine_list_rev (Datatypes.length varctxt) [];
+        PolyLang.pi_transformation := normalize_affine_list_rev (Datatypes.length varctxt) tf;
+        PolyLang.pi_waccess := normalize_access_list_rev (Datatypes.length varctxt) w;
+        PolyLang.pi_raccess := normalize_access_list_rev (Datatypes.length varctxt) r;
+      |}] ipl ->
+    Permutation ipl sorted_ipl ->
+    Sorted PolyLang.instr_point_sched_le sorted_ipl ->
+    PolyLang.instr_point_list_semantics sorted_ipl st1 st2 ->
+    Instr.InitEnv varctxt envv st1 ->
+    exists st2',
+      Loop.loop_semantics (Loop.Instr i es) (rev envv) st1 st2' /\ State.eq st2 st2'.
+Proof.
+    intros i es varctxt envv ipl sorted_ipl st1 st2 tf w r
+      Htf Hacc Hflat Hperm Hsorted Hipls Hinit.
+    pose proof (Instr.init_env_samelen varctxt envv st1 Hinit) as Hlen.
+    assert (affine_product (normalize_affine_list_rev (Datatypes.length varctxt) tf) envv =
+            map (Loop.eval_expr (rev envv)) es) as Haff.
+    {
+      eapply exprlist_to_aff_rev_normalized_correct; eauto.
+    }
+    eapply flatten_instrs_singleton_inv in Hflat.
+    eapply flatten_instr_nth_depth0_emptydom_singleton in Hflat.
+    2: reflexivity.
+    2: simpl; reflexivity.
+    destruct Hflat as (ip0 & Hipl & Hnth & Hidx & Htr & Hts & Hinstr & Hdep).
+    subst ipl.
+    eapply permutation_singleton in Hperm.
+    subst sorted_ipl.
+    eapply instr_point_list_semantics_singleton_inv in Hipls.
+    destruct Hipls as (stmid & Hipsema & Heq).
+    inversion Hipsema as [wcs rcs Hipinstr]; clear Hipsema.
+    assert (affine_product (PolyLang.ip_transformation ip0) (PolyLang.ip_index ip0) =
+            map (Loop.eval_expr (rev envv)) es) as Hargs_rev.
+    {
+      rewrite Htr.
+      rewrite Hidx.
+      replace (Datatypes.length varctxt + 0)%nat with (Datatypes.length varctxt) by lia.
+      exact Haff.
+    }
+    rewrite Hargs_rev in Hipinstr.
+    rewrite Hinstr in Hipinstr.
+    exists stmid.
+    split.
+    - eapply Loop.LInstr.
+      eauto.
+    - eapply State.eq_sym.
+      exact Heq.
+Qed.
+
+Lemma extract_stmt_to_loop_semantics_core:
+    forall stmt varctxt vars pis envv ipl sorted_ipl st1 st2,
+    wf_scop_stmt stmt = true ->
+    extract_stmt stmt [] (Datatypes.length varctxt) 0 [] = Okk pis ->
+    check_extracted_wf pis varctxt vars = true ->
+    PolyLang.flatten_instrs envv pis ipl ->
+    Permutation ipl sorted_ipl ->
+    Sorted PolyLang.instr_point_sched_le sorted_ipl ->
+    PolyLang.instr_point_list_semantics sorted_ipl st1 st2 ->
+    Instr.Compat vars st1 ->
+    Instr.NonAlias st1 ->
+    Instr.InitEnv varctxt envv st1 ->
+    exists st2',
+      Loop.loop_semantics stmt (rev envv) st1 st2' /\ State.eq st2 st2'.
+Proof.
+    intros stmt varctxt vars pis envv ipl sorted_ipl st1 st2
+      Hwf Hextract Hchk Hflat Hperm Hsorted Hipls Hcompat Hnonalias Hinit.
+    destruct stmt as [lb ub body | i es | stmts | test body].
+    2:{
+      eapply extract_stmt_instr_success_inv in Hextract.
+      destruct Hextract as (tf & w & r & Htf & Hacc & Hpis).
+      subst pis.
+      replace (Datatypes.length varctxt + 0)%nat with (Datatypes.length varctxt) in Htf by lia.
+      replace (Datatypes.length varctxt + 0)%nat with (Datatypes.length varctxt) in Hflat by lia.
+      replace (Datatypes.length varctxt + 0)%nat with (Datatypes.length varctxt) in Hchk by lia.
+      eapply (instr_branch_core i es varctxt envv ipl sorted_ipl st1 st2 tf w r); eauto.
+    }
+Admitted.
 
 
 (* Lemma extract_stmt_correct: 
@@ -449,12 +1815,33 @@ Theorem extractor_correct:
     exists st2',
     Loop.semantics loop st1 st2' /\ State.eq st2 st2'.
 Proof.
-    intros. unfold extractor in H.
+    intros loop pol st1 st2 Hext Hsema.
     destruct loop as [[stmt varctxt] vars].
-    remember (extract_stmt stmt [] (Datatypes.length varctxt) []) as Extract.
-    destruct Extract; try discriminate.
-    inv H. rename l into pol.
-Admitted.
+    assert (Hscop: wf_scop_stmt stmt = true).
+    { eapply extractor_success_implies_wf_scop; eauto. }
+    eapply extractor_success_inv in Hext.
+    destruct Hext as [pis [Hextract [Hwf Hpol]]].
+    subst pol.
+    eapply instance_list_semantics_inv in Hsema.
+    destruct Hsema as (pis0 & varctxt0 & vars0 & envv &
+      Hpprog & Hcompat & Hnonalias & Hinitenv & Hpolysema).
+    inversion Hpprog; subst; clear Hpprog.
+    eapply poly_instance_list_semantics_inv in Hpolysema.
+    destruct Hpolysema as (pis1 & varctxt1 & vars1 & ipl & sorted_ipl &
+      Hpprog' & Hflatten & Hperm & Hsorted & Hipls).
+    inversion Hpprog'; subst; clear Hpprog'.
+    pose proof (
+      extract_stmt_to_loop_semantics_core
+        _ _ _ _ _ _ _ _ _
+        Hscop Hextract Hwf Hflatten Hperm Hsorted Hipls
+        Hcompat Hnonalias Hinitenv
+    ) as Hcore.
+    destruct Hcore as (st2' & Hloop & Heq).
+    exists st2'.
+    split.
+    - eapply loop_semantics_intro_from_envv; eauto.
+    - exact Heq.
+Qed.
 
 
 End Extractor.
